symmetric neg exp

theories/eris/examples/neg_exp.v
@@ -2785,7 +2785,7 @@ Section program.
 
   Definition NegExpSymm : val :=
     λ: "e",
-      let: "v" := NegExp #() in
+      let: "v" := NegExp #(Z.of_nat 0) in
       let: "b" := rand (#1) in
       ("b", "v").
 
@@ -3057,66 +3057,273 @@ Section AccuracyBound.
 End AccuracyBound.
 
 
-(*
-
-
-Section spec.
-  Context `{!erisGS Σ}.
+Section Symmetric.
   Import Hierarchy.
+  Context `{!erisGS Σ}.
 
-  (* Sampler returning N * [0,1] samples *)
-  Context (sampler : val).
-  Context (distrib : nat → R → R).
-  Context (distrib_nn : ∀ n r, r < 0 → distrib n r = 0).
-  Context (spec : ∀ E F M, (∀ x k, 0 <= F x k <= M) → (∀ x1 : nat, PCts (F x1) 0 1) →
-                  ⊢ ↯(SeriesC (fun (k : nat) => RInt (fun x => distrib k x * F k x) 0 1)) -∗
-                     WP sampler #() @ E {{ vp, ∃ k : nat, ∃ r : R, ∃ l : val, lazy_real l r  ∗ ⌜vp = PairV l #k ⌝ ∗ ↯(F k r) }}).
+  Definition NegExpSymm_ρ (_ : fin 2) (k : nat) (x : R) : R :=
+    exp (-(x + k))%R / 2.
 
-  Definition Symm_μ : bool → nat → R → R :=
-    fun b n r => distrib n r / 2.
+  Definition NegExpSymm_CreditV (F : fin 2 → nat → R → R)  :=
+    (SeriesC (fun (b : fin 2) => SeriesC (fun (k : nat) => RInt (fun x => NegExpSymm_ρ b k x * F b k x) 0 1))).
 
-  Theorem SymmCreditV E (F : bool → nat → R → R) M :
-    (∀ x k b, 0 <= F b k x <= M) → (∀ b1 : bool, ∀ x1 : nat, PCts (F b1 x1) 0 1) →
-    ⊢ ↯(SeriesC (fun (b : bool) => SeriesC (fun (k : nat) => RInt (fun x => Symm_μ b k x * F b k x) 0 1))) -∗
-       WP SampleSymmetric sampler @ E
-         {{ vp, ∃ b : fin 2, ∃ k : nat, ∃ r : R, ∃ l : val, lazy_real l r  ∗
-                 ⌜vp = PairV #(fin_to_nat b) (PairV l #k) ⌝ ∗ ↯(F (fin_to_bool b) k r) }}.
+
+  Lemma wp_NegExp_sym E (F : fin 2 → nat → R → R) {M}
+      (Hnn : ∀ c a b, 0 <= b <= 1 → 0 <= F c a b <= M) (HP : ∀ x x1, PCts (F x x1) 0 1)  :
+    ⊢ ↯ (NegExpSymm_CreditV F) -∗
+           WP NegExpSymm #() @ E
+      {{ p, ∃ (b : fin 2) (vz : nat) (vr : R) (ℓ : val),
+            ⌜p = PairV #(fin_to_nat b) (PairV #(Z.of_nat vz) ℓ)⌝ ∗
+            lazy_real ℓ vr ∗ ⌜0 <= vr < 1 ⌝ ∗
+            ↯(F b vz vr)}}.
   Proof.
-    intros HF HC.
     iIntros "Hε".
-    rewrite /SampleSymmetric.
+    rewrite /NegExpSymm.
     wp_pures.
-    wp_bind (sampler _).
+    wp_bind (NegExp _).
     iApply (pgl_wp_mono).
     2: {
-      wp_apply (spec E (fun n r => (F true n r + F false n r) / 2) M).
-      { intros ??.
+      iApply ((@wp_NegExp_gen _ _ E (fun n r => (F (0)%fin n r + F (1)%fin n r) / 2) M) with "[Hε]").
+      { intros ???.
         split.
-        { admit. }
-        { admit. }
+        { apply Rcomplements.Rdiv_le_0_compat; try lra.
+          apply Rplus_le_le_0_compat.
+          { apply Hnn. lra. }
+          { apply Hnn. lra. }
+        }
+        { suffices  ? :  (F 0%fin a b + F 1%fin a b) <= M + M by lra.
+          apply Rplus_le_compat.
+          { apply Hnn. lra. }
+          { apply Hnn. lra. }
+        }
       }
-      { admit. }
+      { intros ?.
+        replace (λ r : R, (F 0%fin x1 r + F 1%fin x1 r) / 2)
+          with (λ r : R, F 0%fin x1 r * / 2 + F 1%fin x1 r * / 2).
+        2: (funexti; lra).
+        apply PCts_plus.
+        { apply PCts_mult; [apply HP|].
+          apply PCts_cts. intros ??. apply Continuity.continuous_const.
+        }
+        { apply PCts_mult; [apply HP|].
+          apply PCts_cts. intros ??. apply Continuity.continuous_const.
+        }
+      }
       { iApply (ec_eq with "Hε").
-        rewrite /Symm_μ.
-        rewrite SeriesC_bool.
+        rewrite /NegExpSymm_CreditV.
+        rewrite SeriesC_fin2.
         rewrite -SeriesC_plus.
-        2: admit.
-        2: admit.
+        2: {
+          rewrite /NegExpSymm_ρ.
+          eapply (ex_seriesC_le _ (λ k : nat, (RInt (λ x : R, exp (- (x + k)) / 2) 0 1) * M)).
+          { intros ?.
+            split.
+            { apply RInt_ge_0; try lra.
+              { apply ex_RInt_mult.
+                { rewrite /NegExpSymm_ρ//=.
+                  apply (ex_RInt_continuous (V := R_CompleteNormedModule)).
+                  intros ??.
+                  apply (Derive.ex_derive_continuous (V := R_CompleteNormedModule)).
+                  by auto_derive.
+                }
+                { apply PCts_RInt, HP. }
+              }
+              { intros ??.
+                apply Rmult_le_pos.
+                {  apply Rcomplements.Rdiv_le_0_compat; try lra.
+                   apply Rexp_nn.
+                }
+                { apply Hnn; lra. }
+              }
+            }
+            { rewrite RInt_Rmult'.
+              2: {
+                apply (ex_RInt_continuous (V := R_CompleteNormedModule)).
+                intros ??.
+                apply (Derive.ex_derive_continuous (V := R_CompleteNormedModule)).
+                by auto_derive.
+              }
+              apply RInt_le; try lra.
+              { apply ex_RInt_mult.
+                { rewrite /NegExpSymm_ρ//=.
+                  apply (ex_RInt_continuous (V := R_CompleteNormedModule)).
+                  intros ??.
+                  apply (Derive.ex_derive_continuous (V := R_CompleteNormedModule)).
+                  by auto_derive.
+                }
+                { apply PCts_RInt, HP. }
+              }
+              { apply ex_RInt_mult.
+                { rewrite /NegExpSymm_ρ//=.
+                  apply (ex_RInt_continuous (V := R_CompleteNormedModule)).
+                  intros ??.
+                  apply (Derive.ex_derive_continuous (V := R_CompleteNormedModule)).
+                  by auto_derive.
+                }
+                { apply ex_RInt_const. }
+              }
+              { intros ??.
+                apply Rmult_le_compat_l; [|apply Hnn; lra].
+                apply Rcomplements.Rdiv_le_0_compat; try lra.
+                apply Rexp_nn.
+              }
+            }
+          }
+          { apply ex_seriesC_scal_r.
+            apply (ex_seriesC_RInt (fun n => exp (-n) * / 2)); try lra.
+            { intros ???.
+              apply Rcomplements.Rdiv_le_0_compat; try lra.
+              apply Rexp_nn.
+            }
+            { apply ex_seriesC_scal_r.
+              apply ex_exp_geo_series. }
+            { intros ???.
+              rewrite Rabs_right.
+              2: { apply Rle_ge.
+                   apply Rcomplements.Rdiv_le_0_compat; try lra.
+                   apply Rexp_nn.
+              }
+              { rewrite Rdiv_def.
+                apply Rmult_le_compat_r; try lra.
+                apply exp_mono.
+                apply Ropp_le_contravar.
+                have ? := pos_INR n. lra.
+              }
+            }
+            { intros ?.
+              apply (ex_RInt_continuous (V := R_CompleteNormedModule)).
+              intros ??.
+              apply (Derive.ex_derive_continuous (V := R_CompleteNormedModule)).
+              by auto_derive.
+            }
+          }
+        }
+        2: {
+          rewrite /NegExpSymm_ρ.
+          eapply (ex_seriesC_le _ (λ k : nat, (RInt (λ x : R, exp (- (x + k)) / 2) 0 1) * M)).
+          { intros ?.
+            split.
+            { apply RInt_ge_0; try lra.
+              { apply ex_RInt_mult.
+                { rewrite /NegExpSymm_ρ//=.
+                  apply (ex_RInt_continuous (V := R_CompleteNormedModule)).
+                  intros ??.
+                  apply (Derive.ex_derive_continuous (V := R_CompleteNormedModule)).
+                  by auto_derive.
+                }
+                { apply PCts_RInt, HP. }
+              }
+              { intros ??.
+                apply Rmult_le_pos.
+                {  apply Rcomplements.Rdiv_le_0_compat; try lra.
+                   apply Rexp_nn.
+                }
+                { apply Hnn; lra. }
+              }
+            }
+            { rewrite RInt_Rmult'.
+              2: {
+                apply (ex_RInt_continuous (V := R_CompleteNormedModule)).
+                intros ??.
+                apply (Derive.ex_derive_continuous (V := R_CompleteNormedModule)).
+                by auto_derive.
+              }
+              apply RInt_le; try lra.
+              { apply ex_RInt_mult.
+                { rewrite /NegExpSymm_ρ//=.
+                  apply (ex_RInt_continuous (V := R_CompleteNormedModule)).
+                  intros ??.
+                  apply (Derive.ex_derive_continuous (V := R_CompleteNormedModule)).
+                  by auto_derive.
+                }
+                { apply PCts_RInt, HP. }
+              }
+              { apply ex_RInt_mult.
+                { rewrite /NegExpSymm_ρ//=.
+                  apply (ex_RInt_continuous (V := R_CompleteNormedModule)).
+                  intros ??.
+                  apply (Derive.ex_derive_continuous (V := R_CompleteNormedModule)).
+                  by auto_derive.
+                }
+                { apply ex_RInt_const. }
+              }
+              { intros ??.
+                apply Rmult_le_compat_l; [|apply Hnn; lra].
+                apply Rcomplements.Rdiv_le_0_compat; try lra.
+                apply Rexp_nn.
+              }
+            }
+          }
+          { apply ex_seriesC_scal_r.
+            apply (ex_seriesC_RInt (fun n => exp (-n) * / 2)); try lra.
+            { intros ???.
+              apply Rcomplements.Rdiv_le_0_compat; try lra.
+              apply Rexp_nn.
+            }
+            { apply ex_seriesC_scal_r.
+              apply ex_exp_geo_series. }
+            { intros ???.
+              rewrite Rabs_right.
+              2: { apply Rle_ge.
+                   apply Rcomplements.Rdiv_le_0_compat; try lra.
+                   apply Rexp_nn.
+              }
+              { rewrite Rdiv_def.
+                apply Rmult_le_compat_r; try lra.
+                apply exp_mono.
+                apply Ropp_le_contravar.
+                have ? := pos_INR n. lra.
+              }
+            }
+            { intros ?.
+              apply (ex_RInt_continuous (V := R_CompleteNormedModule)).
+              intros ??.
+              apply (Derive.ex_derive_continuous (V := R_CompleteNormedModule)).
+              by auto_derive.
+            }
+          }
+        }
+        rewrite /NegExp_CreditV.
         apply SeriesC_ext.
         intros n.
         rewrite RInt_add.
-        2: admit.
-        2: admit.
+        2: {
+          apply ex_RInt_mult.
+          { rewrite /NegExpSymm_ρ//=.
+            apply (ex_RInt_continuous (V := R_CompleteNormedModule)).
+            intros ??.
+            apply (Derive.ex_derive_continuous (V := R_CompleteNormedModule)).
+            by auto_derive.
+          }
+          { apply PCts_RInt, HP. }
+        }
+        2: {
+          apply ex_RInt_mult.
+          { rewrite /NegExpSymm_ρ//=.
+            apply (ex_RInt_continuous (V := R_CompleteNormedModule)).
+            intros ??.
+            apply (Derive.ex_derive_continuous (V := R_CompleteNormedModule)).
+            by auto_derive.
+          }
+          { apply PCts_RInt, HP. }
+        }
         apply RInt_ext.
         intros ??.
+        rewrite /NegExpSymm_ρ//=.
+        rewrite /NegExp_ρ/NegExp_ρ0//=.
+        rewrite Iverson_True.
+        2: { lia. }
+        rewrite Iverson_True.
+        2: { rewrite /Icc. lra. }
+        rewrite Nat.sub_0_r.
         lra.
       }
     }
     simpl.
-    iIntros (v) "[%k [%r [%l [Hr [-> Hec]]]]]".
+    iIntros (v) "[%k [%r [%l [-> [Hr [% Hec]]]]]]".
     wp_pures.
-    wp_apply (wp_couple_rand_adv_comp _ _ _ _ (fun (s : fin 2) => F (fin_to_bool s) k r) with "Hec").
-    { intros n. apply HF. }
+    wp_apply (wp_couple_rand_adv_comp _ _ _ _ (fun (s : fin 2) => F s k r) with "Hec").
+    { intros n. apply Hnn. lra. }
     { rewrite SeriesC_fin2 //=. lra. }
     iIntros (b) "Hec".
     wp_pures.
@@ -3124,7 +3331,6 @@ Section spec.
     iExists b, k, r, l.
     iFrame.
     iPureIntro; done.
-  Admitted.
+  Qed.
 
-End spec.
-*)
+End Symmetric.
